isabelle/AbstractBindingTrees.thy
@@ -2,7 +2,7 @@ theory AbstractBindingTrees
   imports Main ABT Rename
 begin
 
-abbreviation shift :: "('op ABT) sub" ("\<up>") where
+definition shift :: "('op ABT) sub" ("\<up>") where
   "\<up> x \<equiv> Var (Suc x)"
 
 abbreviation shift_many :: "nat \<Rightarrow> ('op ABT) sub" ("\<up>") where
@@ -12,14 +12,17 @@ interpretation abt_s: substable "Var 0" "rename Suc" "Var" "\<lambda> x. x"
   apply unfold_locales
   apply (auto simp add: rename_def)
   done
- 
-definition exts :: "('op ABT) sub \<Rightarrow> ('op ABT) sub" where
-  "exts \<sigma> \<equiv> abt_s.ext \<sigma>"
+
+definition ext :: "('op ABT) sub \<Rightarrow> ('op ABT) sub" where
+  "ext \<sigma> \<equiv> abt_s.extend \<sigma>"
 
 definition subst :: "('op ABT) sub \<Rightarrow> 'op ABT \<Rightarrow> 'op ABT" ("\<llangle>_\<rrangle>") where
   "\<llangle> \<sigma> \<rrangle> \<equiv> abt_s.map_abt \<sigma>"
 
-abbreviation ren_sub :: "var sub \<Rightarrow> ('op ABT) sub" ("\<lceil>_\<rceil>") where
+definition subst_arg :: "('op ABT) sub \<Rightarrow> 'op Arg \<Rightarrow> 'op Arg" ("\<llangle>_\<rrangle>\<^sub>a") where
+  "\<llangle> \<sigma> \<rrangle>\<^sub>a \<equiv> abt_s.map_arg \<sigma>"
+
+definition ren_sub :: "var sub \<Rightarrow> ('op ABT) sub" ("\<lceil>_\<rceil>") where
   "\<lceil>\<rho>\<rceil> x \<equiv> Var (\<rho> x)"
 
 definition seqss :: "('op ABT) sub \<Rightarrow> ('op ABT) sub \<Rightarrow> ('op ABT) sub" (infixr ";" 70) where
@@ -62,6 +65,18 @@ theorem TailCons[simp]: "(M \<bullet> \<sigma>) (Suc x) = \<sigma> x"
 theorem TailConsSub[simp]: "\<llangle>M \<bullet> \<sigma>\<rrangle> (Var (Suc x)) = \<sigma> x"
   unfolding subst_def by simp
 
+theorem VarSub: "\<llangle>\<sigma>\<rrangle> (Var x) = \<sigma> x"
+  unfolding subst_def by simp
+
+theorem AppSub[simp]: "\<llangle>\<sigma>\<rrangle> (App op args) = App op (map (\<llangle>\<sigma>\<rrangle>\<^sub>a) args)"
+  by (simp add: subst_def subst_arg_def)
+
+theorem TrmSub[simp]: "\<llangle>\<sigma>\<rrangle>\<^sub>a (Trm M) = Trm (\<llangle>\<sigma>\<rrangle> M)"
+  by (simp add: subst_def subst_arg_def)
+
+theorem BndSub[simp]: "\<llangle>\<sigma>\<rrangle>\<^sub>a (Bnd A) = Bnd (\<llangle>ext \<sigma>\<rrangle>\<^sub>a A)"
+  by (simp add: ext_def subst_arg_def)
+
 theorem ShiftCons[simp]: "\<up> ; (M \<bullet> \<sigma>) = \<sigma>"
   unfolding cons_def subst_def seqss_def shift_def by simp
 
@@ -100,46 +115,45 @@ interpretation ren_sub:
   by unfold_locales auto
 
 lemma cong_ext:
- "ren_sub.cong \<sigma> \<tau> \<Longrightarrow> ren_sub.cong (extr \<sigma>) (exts \<tau>)"
+ "ren_sub.cong \<sigma> \<tau> \<Longrightarrow> ren_sub.cong (extr \<sigma>) (ext \<tau>)"
 proof clarify
   fix x
   assume st: "ren_sub.cong \<sigma> \<tau>" 
-  show "\<lceil>extr \<sigma>\<rceil> x = (exts \<tau>) x" 
+  show "Var (extr \<sigma> x) = (ext \<tau>) x"
   proof (cases x)
     case 0
-    then show ?thesis unfolding exts_def by simp
+    then show ?thesis unfolding ext_def by simp
   next
     case (Suc y)
-    with Suc have "\<lceil>extr \<sigma>\<rceil> x = Var (Suc (\<sigma> y))" by (simp add: cons_def seqrr_def)
+    with Suc have "Var (extr \<sigma> x) = Var (Suc (\<sigma> y))" by (simp add: cons_def seqrr_def)
     also have "... = rename Suc (Var (\<sigma> y))" unfolding rename_def by simp
     also have "... = rename Suc (\<tau> y)" using st by simp
-    also have "... = exts \<tau> x" using Suc unfolding exts_def by (simp add: cons_def)
+    also have "... = ext \<tau> x" using Suc unfolding ext_def by (simp add: cons_def)
     finally show ?thesis .
   qed  
 qed
 
 theorem rename_subst: "rename \<rho> M = \<llangle> \<lceil> \<rho> \<rceil> \<rrangle> M"
 proof -
-  have 1: "ren_sub.cong \<rho> \<lceil>\<rho>\<rceil>" by auto
+  have 1: "ren_sub.cong \<rho> \<lceil>\<rho>\<rceil>" unfolding ren_sub_def by auto
   from 1 cong_ext have "var_s.map_abt \<rho> M = abt_s.map_abt \<lceil>\<rho>\<rceil> M" 
-    unfolding extr_def exts_def apply (rule ren_sub.map_cong) by simp
+    unfolding extr_def ext_def apply (rule ren_sub.map_cong) by simp
   then show ?thesis unfolding subst_def rename_def by auto
 qed
 
+ (*
 lemma lift_seq_up: "abt_s.lift_sub \<sigma> = \<sigma> ; \<up>"
   apply (rule ext)
-  unfolding seqss_def shift_def using rename_subst[of Suc] apply auto done
+  unfolding seqss_def shift_def  using rename_subst[of Suc] apply auto done
+*)
 
-lemma ren_suc_shift: "\<lceil>Suc\<rceil> = \<up>"
-  unfolding shift_def by simp
-
-lemma exts_cons_seq: "exts \<sigma> = Var 0 \<bullet> (\<sigma> ; \<up>)"
+lemma ext_cons_seq: "ext \<sigma> = Var 0 \<bullet> (\<sigma> ; \<up>)"
 proof -
   have 1: "(\<lambda> x. rename Suc (\<sigma> x)) = (\<lambda> x. \<llangle> \<lceil> Suc \<rceil> \<rrangle> (\<sigma> x))"
     using rename_subst[of Suc] by auto
-  have "exts \<sigma> = Var 0 \<bullet> (\<lambda> x. \<llangle> \<lceil> Suc \<rceil> \<rrangle> (\<sigma> x))" using 1 unfolding exts_def by simp
-  also have "... = Var 0 \<bullet> (\<sigma> ; \<up>)" unfolding seqss_def by simp
-  finally show "exts \<sigma> = Var 0 \<bullet> (\<sigma> ; \<up>)" .
+  have "ext \<sigma> = Var 0 \<bullet> (\<lambda> x. \<llangle> \<lceil> Suc \<rceil> \<rrangle> (\<sigma> x))" using 1 unfolding ext_def by simp
+  also have "... = Var 0 \<bullet> (\<sigma> ; \<up>)" unfolding seqss_def shift_def ren_sub_def by simp
+  finally show "ext \<sigma> = Var 0 \<bullet> (\<sigma> ; \<up>)" .
 qed
 
 interpretation rss:
@@ -155,11 +169,11 @@ theorem assoc_RRS[simp]: "(\<rho> r;r \<sigma>) r; \<tau> = \<rho> r; (\<sigma> 
 theorem assoc_RSS[simp]: "(\<rho> r; \<sigma>) ; \<tau> = \<rho> r; (\<sigma> ; \<tau>)"
   unfolding seqrs_def seqss_def by auto
 
-lemma rss_comp_cong_ext: assumes 1: "\<rho> r; \<sigma> = \<tau>" shows "(extr \<rho>) r; (exts \<sigma>) = (exts \<tau>)"
-proof (simp add: exts_cons_seq)
-  have "Var 0 \<bullet> (\<rho> r; \<sigma> ; \<lceil>Suc\<rceil>) = Var 0 \<bullet> ((\<rho> r; \<sigma>) ; \<lceil>Suc\<rceil>)" by simp
-  also have "... = Var 0 \<bullet> (\<tau> ; \<lceil>Suc\<rceil>)" using 1 by simp
-  finally show "Var 0 \<bullet> (\<rho> r; \<sigma> ; \<lceil>Suc\<rceil>) = Var 0 \<bullet> (\<tau> ; \<lceil>Suc\<rceil>)" .
+lemma rss_comp_cong_ext: assumes 1: "\<rho> r; \<sigma> = \<tau>" shows "(extr \<rho>) r; (ext \<sigma>) = (ext \<tau>)"
+proof (simp add: ext_cons_seq)
+  have "Var 0 \<bullet> (\<rho> r; \<sigma> ; \<up>) = Var 0 \<bullet> ((\<rho> r; \<sigma>) ; \<up>)" unfolding shift_def by simp
+  also have "... = Var 0 \<bullet> (\<tau> ; \<up>)" using 1 by simp
+  finally show "Var 0 \<bullet> (\<rho> r; \<sigma> ; \<up>) = Var 0 \<bullet> (\<tau> ; \<up>)" .
 qed
 
 lemma rsscc_eq_seqrs: "(\<rho> r; \<sigma> = \<tau>) = (rss.comp_cong \<sigma> \<rho> \<tau>)" 
@@ -174,21 +188,21 @@ proof -
     fix \<sigma>::"var sub" and \<tau> :: "('op ABT) sub" and \<rho> x
     assume 4: "rss.comp_cong \<tau> \<sigma> \<rho>"
     then have "\<sigma> r; \<tau> = \<rho>" using rsscc_eq_seqrs by fast
-    then have 1: "(extr \<sigma>) r; (exts \<tau>) = (exts \<rho>)"
+    then have 1: "(extr \<sigma>) r; (ext \<tau>) = (ext \<rho>)"
       by (rule rss_comp_cong_ext) 
-    have "rss.comp_cong (abt_s.ext \<tau>) (var_s.ext \<sigma>) (abt_s.ext \<rho>)"
+    have "rss.comp_cong (abt_s.extend \<tau>) (var_s.extend \<sigma>) (abt_s.extend \<rho>)"
       apply auto apply (case_tac x) apply force 
     proof -
       fix x
-      have "(extr \<sigma> r; exts \<tau>) x = (exts \<rho>) x " using 1 by auto
-      then show "abt_s.ext \<tau> (var_s.ext \<sigma> x) = abt_s.ext \<rho> x"
-        unfolding extr_def exts_def seqrs_def .
+      have "(extr \<sigma> r; ext \<tau>) x = (ext \<rho>) x " using 1 by auto
+      then show "abt_s.extend \<tau> (var_s.extend \<sigma> x) = abt_s.extend \<rho> x"
+        unfolding extr_def ext_def seqrs_def .
     qed      
   }
-  then have 3: "\<forall>\<sigma> \<tau> \<rho>. rss.comp_cong \<tau> \<sigma> \<rho> \<longrightarrow> rss.comp_cong (exts \<tau>) (var_s.ext \<sigma>) (exts \<rho>)"
-    unfolding exts_def by blast
+  then have 3: "\<forall>\<sigma> \<tau> \<rho>. rss.comp_cong \<tau> \<sigma> \<rho> \<longrightarrow> rss.comp_cong (ext \<tau>) (var_s.extend \<sigma>) (ext \<rho>)"
+    unfolding ext_def by blast
   from 2 3 have "abt_s.map_abt \<sigma> (var_s.map_abt \<rho> M) = abt_s.map_abt \<tau> M"
-    unfolding exts_def by (rule rss.map_fusion)
+    unfolding ext_def by (rule rss.map_fusion)
   then show ?thesis unfolding subst_def rename_def by simp  
 qed
 
@@ -209,22 +223,22 @@ lemma srscc_eq_seqsr: "(\<sigma> ;r \<rho> = \<tau>) = (srs.comp_cong \<rho> \<s
 
 lemma srs_comp_cong_ext: fixes x :: var
   assumes cc: "\<sigma> ;r \<rho> = \<tau>"
-  shows "rename (extr \<rho>) (exts \<sigma> x) = exts \<tau> x"
+  shows "rename (extr \<rho>) (ext \<sigma> x) = ext \<tau> x"
 proof (cases x)
   case 0
-  then show ?thesis unfolding exts_def by simp 
+  then show ?thesis unfolding ext_def by simp 
 next
   case (Suc y)
-  have            "((exts \<sigma>) ;r (extr \<rho>)) x 
-                 = rename (extr \<rho>) (rename Suc (\<sigma> y))" using Suc seqsr_def unfolding exts_def by auto
+  have            "((ext \<sigma>) ;r (extr \<rho>)) x 
+                 = rename (extr \<rho>) (rename Suc (\<sigma> y))" using Suc seqsr_def unfolding ext_def by auto
   also have "... = rename (Suc r;r (extr \<rho>)) (\<sigma> y)" 
     by (rule rename_fusion[of "(extr \<rho>)" Suc "\<sigma> y"])
   also have "... = rename (\<rho> r;r Suc) (\<sigma> y)" by simp
   also have "... = rename Suc (rename \<rho> (\<sigma> y))" using rename_fusion[of Suc \<rho> "\<sigma> y"] by auto
   also have "... = rename Suc ((\<sigma> ;r \<rho>) y)" unfolding seqsr_def ..
   also have "... = rename Suc (\<tau> y)" using cc by simp
-  also have "... = exts \<tau> x" using Suc unfolding exts_def by (simp add: cons_def)
-  finally have "((exts \<sigma>) ;r (extr \<rho>)) x = exts \<tau> x" unfolding exts_def by simp
+  also have "... = ext \<tau> x" using Suc unfolding ext_def by (simp add: cons_def)
+  finally have "((ext \<sigma>) ;r (extr \<rho>)) x = ext \<tau> x" unfolding ext_def by simp
   then show ?thesis unfolding seqsr_def by simp
 qed
 
@@ -238,9 +252,9 @@ proof -
   proof (rule srs.map_fusion, clarify)
     fix \<sigma> \<tau> \<rho> x assume "srs.comp_cong \<tau> \<sigma> \<rho>"
     then have "\<sigma> ;r \<tau> = \<rho>" unfolding seqsr_def rename_def by auto
-    then have "rename (extr \<tau>) (exts \<sigma> x) = exts \<rho> x" by (rule srs_comp_cong_ext)
-    then show "var_s.map_abt (var_s.ext \<tau>) (abt_s.ext \<sigma> x) = abt_s.ext \<rho> x"
-      unfolding rename_def extr_def exts_def by fast
+    then have "rename (extr \<tau>) (ext \<sigma> x) = ext \<rho> x" by (rule srs_comp_cong_ext)
+    then show "var_s.map_abt (var_s.extend \<tau>) (abt_s.extend \<sigma> x) = abt_s.extend \<rho> x"
+      unfolding rename_def extr_def ext_def by fast
   qed
   then show "rename \<rho> (\<llangle>\<sigma>\<rrangle> M) = \<llangle>\<sigma> ;r \<rho>\<rrangle> M"
     unfolding rename_def subst_def by fast
@@ -273,20 +287,20 @@ lemma seqss_eq_ssscc: "(sss.comp_cong \<rho> \<sigma> \<tau>) = (\<sigma> ; \<rh
 lemma sss_comp_cong_ext:
   fixes x :: var
   assumes 1: "(\<sigma> ; \<rho>) = \<tau>"
-  shows "((exts \<sigma>) ; (exts \<rho>)) x = exts \<tau> x"
+  shows "((ext \<sigma>) ; (ext \<rho>)) x = ext \<tau> x"
 proof (cases x)
   case 0
-  then show ?thesis unfolding exts_def by (simp add: subst_def)
+  then show ?thesis unfolding ext_def by (simp add: subst_def)
 next
   case (Suc y)
   thm subst_rename_fusion
-  have "(exts \<sigma> ; exts \<rho>) x = \<llangle>exts \<rho>\<rrangle> (exts \<sigma> x)" unfolding seqss_def by simp
-  also have "... = \<llangle>exts \<rho>\<rrangle> (rename Suc (\<sigma> y))" using Suc unfolding exts_def by simp
-  also have "... = \<llangle>Suc r; exts \<rho>\<rrangle> (\<sigma> y)" by (rule subst_rename_fusion) simp
-  also have "... = \<llangle> \<rho> ;r Suc \<rrangle> (\<sigma> y)" unfolding seqsr_def seqrs_def exts_def by simp  
+  have "(ext \<sigma> ; ext \<rho>) x = \<llangle>ext \<rho>\<rrangle> (ext \<sigma> x)" unfolding seqss_def by simp
+  also have "... = \<llangle>ext \<rho>\<rrangle> (rename Suc (\<sigma> y))" using Suc unfolding ext_def by simp
+  also have "... = \<llangle>Suc r; ext \<rho>\<rrangle> (\<sigma> y)" by (rule subst_rename_fusion) simp
+  also have "... = \<llangle> \<rho> ;r Suc \<rrangle> (\<sigma> y)" unfolding seqsr_def seqrs_def ext_def by simp  
   also have "... = rename Suc (\<llangle>\<rho>\<rrangle> (\<sigma> y))" using rename_subst_fusion[of Suc \<rho> "\<sigma> y"] by simp
   also have "... = rename Suc (\<tau> y)" using 1 unfolding seqss_def by auto
-  also have "... = exts \<tau> x" using Suc unfolding exts_def by (simp add: cons_def)
+  also have "... = ext \<tau> x" using Suc unfolding ext_def by (simp add: cons_def)
   finally show ?thesis .
 qed
 
@@ -297,9 +311,9 @@ proof -
   proof (rule sss.map_fusion, clarify)
     fix \<sigma> \<tau> \<rho> x assume "sss.comp_cong \<tau> \<sigma> \<rho>"
     then have "\<sigma> ; \<tau> = \<rho>" using seqss_eq_ssscc[of \<tau> \<sigma> \<rho>] by simp
-    then have "((exts \<sigma>) ; (exts \<tau>)) x = exts \<rho> x" by (rule sss_comp_cong_ext)
-    then show "abt_s.map_abt (abt_s.ext \<tau>) (abt_s.ext \<sigma> x) = abt_s.ext \<rho> x" 
-      unfolding seqss_def subst_def exts_def by simp
+    then have "((ext \<sigma>) ; (ext \<tau>)) x = ext \<rho> x" by (rule sss_comp_cong_ext)
+    then show "abt_s.map_abt (abt_s.extend \<tau>) (abt_s.extend \<sigma> x) = abt_s.extend \<rho> x" 
+      unfolding seqss_def subst_def ext_def by simp
   qed
   then show ?thesis unfolding subst_def by simp
 qed
@@ -315,45 +329,105 @@ proof (rule ext)
   finally show "((\<sigma> ; \<tau>) ; \<rho>) x = (\<sigma> ; \<tau> ; \<rho>) x" .
 qed
 
-declare exts_cons_seq[simp]
+declare ext_cons_seq[simp]
 
-theorem subst_commute: "(\<llangle> exts \<sigma>\<rrangle> N) [ \<llangle> \<sigma> \<rrangle> M ] = \<llangle> \<sigma> \<rrangle> (N [ M ])"
+theorem subst_commute: "(\<llangle> ext \<sigma>\<rrangle> N) [ \<llangle> \<sigma> \<rrangle> M ] = \<llangle> \<sigma> \<rrangle> (N [ M ])"
   by simp
 
-theorem commute_subst: " \<llangle> \<sigma> \<rrangle> (N [ M ]) = (\<llangle> exts \<sigma>\<rrangle> N) [ \<llangle> \<sigma> \<rrangle> M ]"
+theorem commute_subst: " \<llangle> \<sigma> \<rrangle> (N [ M ]) = (\<llangle> ext \<sigma>\<rrangle> N) [ \<llangle> \<sigma> \<rrangle> M ]"
   using subst_commute by simp
-
 
 lemma rename_subst_cons[simp]: "\<lceil>y \<bullet> \<rho>\<rceil> = Var y \<bullet> \<lceil>\<rho>\<rceil>"
   apply (rule ext) 
   apply (case_tac x)
-   apply simp
+   unfolding ren_sub_def apply simp
   apply simp
   done
 
 lemma rename_subst_seq[simp]: "\<lceil>\<rho> r;r \<sigma>\<rceil> = \<lceil>\<rho>\<rceil> ; \<lceil>\<sigma>\<rceil>"
 proof (rule ext)
   fix x
-  have "\<lceil>\<rho> r;r \<sigma>\<rceil> x = Var (\<sigma> (\<rho> x))" unfolding seqrr_def by simp
-  also have "... = \<llangle>\<lceil>\<sigma>\<rceil>\<rrangle> (Var (\<rho> x))" unfolding subst_def by simp
-  also have "... = \<llangle>\<lceil>\<sigma>\<rceil>\<rrangle> (\<lceil>\<rho>\<rceil> x)" by simp
+  have "\<lceil>\<rho> r;r \<sigma>\<rceil> x = Var (\<sigma> (\<rho> x))" unfolding seqrr_def ren_sub_def by simp
+  also have "... = \<llangle>\<lceil>\<sigma>\<rceil>\<rrangle> (Var (\<rho> x))" unfolding subst_def ren_sub_def by simp
+  also have "... = \<llangle>\<lceil>\<sigma>\<rceil>\<rrangle> (\<lceil>\<rho>\<rceil> x)" unfolding ren_sub_def by simp
   also have "... = (\<lceil>\<rho>\<rceil> ; \<lceil>\<sigma>\<rceil>) x" unfolding seqss_def by simp
   finally show "\<lceil>\<rho> r;r \<sigma>\<rceil> x = (\<lceil>\<rho>\<rceil> ; \<lceil>\<sigma>\<rceil>) x" .
 qed
 
 declare rename_subst[simp]
 
+theorem ren_suc_shift[simp]: "\<lceil>Suc\<rceil> = \<up>"
+  unfolding shift_def ren_sub_def by simp
+
 theorem rename_subst_commute: "(rename (extr \<rho>) N) [ rename \<rho> M ] = rename \<rho> (N[M])"
-  by simp 
+  by simp
 
 definition subst_two :: "'op ABT \<Rightarrow> 'op ABT \<Rightarrow> 'op ABT" ("_\<lbrace>_\<rbrace>" 60) where
- "N \<lbrace> M \<rbrace> = \<llangle> exts (M \<bullet> \<iota>) \<rrangle> N"
+ "N \<lbrace> M \<rbrace> = \<llangle> ext (M \<bullet> \<iota>) \<rrangle> N"
 declare subst_two_def[simp]
 
 theorem substitution: "M[N][L] = M\<lbrace>L\<rbrace>[N[L]]"
   by simp
 
-theorem exts_sub_cons: "(\<llangle>exts \<sigma>\<rrangle> N)[V] = \<llangle>V \<bullet> \<sigma>\<rrangle> N" 
+theorem ext_sub_cons: "(\<llangle>ext \<sigma>\<rrangle> N)[V] = \<llangle>V \<bullet> \<sigma>\<rrangle> N" 
   by simp
+
+context abt_predicate
+begin
+
+  definition sub_pres :: "('op ABT) sub \<Rightarrow> 't list \<Rightarrow> 't list \<Rightarrow> bool" ("_:_\<rightharpoonup>_" 55) where
+    "\<sigma> : \<Gamma> \<rightharpoonup> \<Gamma>' \<equiv> \<forall> x T. nth \<Gamma> x = T \<longrightarrow> \<Gamma>' \<turnstile> \<sigma> x : T"
+
+  abbreviation wf_abt_sub_P :: "'t list \<Rightarrow> 'op ABT \<Rightarrow> 't \<Rightarrow> bool" where
+    "wf_abt_sub_P \<Gamma> M T \<equiv> \<forall> \<sigma> \<Gamma>'. \<sigma> : \<Gamma> \<rightharpoonup> \<Gamma>' \<longrightarrow> \<Gamma>' \<turnstile> \<llangle>\<sigma>\<rrangle> M : T"
+
+  abbreviation wf_arg_sub_P :: "'t list \<Rightarrow> 't list \<Rightarrow> 'op Arg \<Rightarrow> 't \<Rightarrow> bool" where
+    "wf_arg_sub_P \<Gamma> Bs A T \<equiv> \<forall> \<sigma> \<Gamma>'. (\<sigma> : \<Gamma> \<rightharpoonup> \<Gamma>') \<longrightarrow> (\<Gamma>' ; Bs \<turnstile>\<^sub>a \<llangle>\<sigma>\<rrangle>\<^sub>a A : T)"
+
+  abbreviation wf_args_sub_P :: "'t list \<Rightarrow> 't list list \<Rightarrow> ('op Arg) list \<Rightarrow> 't list \<Rightarrow> bool" where
+    "wf_args_sub_P \<Gamma> Bss As Ts \<equiv> \<forall> \<sigma> \<Gamma>'. (\<sigma> : \<Gamma> \<rightharpoonup> \<Gamma>') \<longrightarrow> (\<Gamma>' ; Bss \<turnstile>\<^sub>+ map (\<llangle>\<sigma>\<rrangle>\<^sub>a) As : Ts)"
+
+  lemma subst_pres_aux: "(\<Gamma> \<turnstile> M : T \<longrightarrow> wf_abt_sub_P \<Gamma> M T) 
+      \<and> (\<Gamma>; Bss \<turnstile>\<^sub>+ As : Ts \<longrightarrow> wf_args_sub_P \<Gamma> Bss As Ts)
+      \<and> (\<Gamma>; Bs \<turnstile>\<^sub>a A : T \<longrightarrow> wf_arg_sub_P \<Gamma> Bs A T)"
+  proof (induction rule: wf_abt_wf_args_wf_arg.induct)
+    case (wf_var \<Gamma> x T)
+    then show ?case apply clarify unfolding VarSub sub_pres_def by auto
+  next
+    case (wf_app \<Gamma> Bss args Ts op T)
+    then show ?case by auto 
+  next
+    case (wf_trm \<Gamma> M T Bs)
+    then show ?case by auto
+  next
+    case (wf_bnd T' \<Gamma> Bs A T)
+    show ?case apply clarify apply simp
+    proof -
+      fix \<sigma> \<Gamma>'
+      assume sub_ok: "\<sigma> : \<Gamma> \<rightharpoonup> \<Gamma>'"
+      have 1: "Var 0 \<bullet> (\<sigma> ; \<up>) : (T'#\<Gamma>) \<rightharpoonup> (T'#\<Gamma>')" unfolding sub_pres_def apply clarify
+        apply (case_tac x) apply force
+      proof -
+        fix x T y assume x: "x = Suc y"
+        have "\<Gamma>' \<turnstile> \<sigma> y : \<Gamma> ! y" using sub_ok sub_pres_def by simp
+        then have "T' # \<Gamma>' \<turnstile> rename Suc (\<sigma> y):\<Gamma> ! y" using shift_pres by blast
+        then have "T' # \<Gamma>' \<turnstile> \<llangle>\<up>\<rrangle> (\<sigma> y):\<Gamma> ! y" by simp
+        then show "T' # \<Gamma>'\<turnstile>(Var 0 \<bullet> (\<sigma> ; \<up>)) x:(T' # \<Gamma>) ! x" 
+          unfolding seqss_def x by simp 
+      qed
+      with wf_bnd.IH show "\<Gamma>';T' # Bs \<turnstile>\<^sub>a Bnd (\<llangle>Var 0 \<bullet> (\<sigma> ; \<up>)\<rrangle>\<^sub>a A) : T" by blast
+    qed
+  next
+    case (wf_nil \<Gamma>)
+    then show ?case by auto
+  next
+    case (wf_cons \<Gamma> Bs A T Bss As Ts)
+    then show ?case by auto
+  qed
+
+  theorem subst_pres: "\<lbrakk> \<Gamma> \<turnstile> M : T; \<sigma> : \<Gamma> \<rightharpoonup> \<Gamma>' \<rbrakk> \<Longrightarrow> \<Gamma>' \<turnstile> \<llangle>\<sigma>\<rrangle> M : T"
+    using subst_pres_aux by blast
+
+end
 
 end
