isabelle/LambdaExample.thy
@@ -4,8 +4,7 @@ begin
 
 section "Lambda Calculus"
 
-datatype op_lam =
-  LamOp | AppOp
+datatype op_lam = LamOp | AppOp
 
 type_synonym Term = "op_lam ABT"
 
@@ -15,8 +14,85 @@ abbreviation Lam :: "Term \<Rightarrow> Term" ("\<lambda>") where
 abbreviation Apply :: "Term \<Rightarrow> Term \<Rightarrow> Term" (infixl "\<cdot>" 60) where
   "L \<cdot> M \<equiv> App AppOp [Trm L, Trm M]"
 
-inductive reduce :: "Term \<Rightarrow> Term \<Rightarrow> bool" (infix "\<longmapsto>" 50) where
-  beta: "(\<lambda> N) \<cdot> M \<longmapsto> N[M]"
+inductive WF_op :: "op_lam \<Rightarrow> unit list list \<Rightarrow> unit list \<Rightarrow> unit \<Rightarrow> bool" where
+  WFLamOp[intro!]: "WF_op LamOp [[()]] [()] ()" |
+  WFAppOp[intro!]: "WF_op AppOp [[],[]] [(),()] ()"
 
+context abt_predicate
+begin
+
+inductive_cases
+  wf_var_elim[elim!]: "\<Gamma> \<turnstile> Var x : T" and
+  wf_app_elim[elim!]: "\<Gamma> \<turnstile> App op args : T" and
+  wf_trm_elim[elim!]: "\<Gamma>; Bs \<turnstile>\<^sub>a Trm M : T" and
+  wf_bnd_elim[elim!]: "\<Gamma>; Bs \<turnstile>\<^sub>a Bnd A : T" and
+  wf_cons_elim[elim!]: "\<Gamma>; Bss \<turnstile>\<^sub>+ As : Ts"
+
+end
+
+interpretation lam: abt_predicate WF_op .
+
+abbreviation WF :: "unit list \<Rightarrow> Term \<Rightarrow> bool" ("_\<turnstile>_") where
+  "\<Gamma> \<turnstile> M \<equiv> lam.wf_abt \<Gamma> M ()"
+
+inductive wf :: "unit list \<Rightarrow> Term \<Rightarrow> bool" where
+  wf_var[intro!]: "nth \<Gamma> x = () \<Longrightarrow> wf \<Gamma> (Var x)" |
+  wf_app[intro!]: "\<lbrakk> wf \<Gamma> L; wf \<Gamma> M \<rbrakk> \<Longrightarrow> wf \<Gamma> (L \<cdot> M)" |
+  wf_abs[intro!]: "wf (()#\<Gamma>) N \<Longrightarrow> wf \<Gamma> (\<lambda> N)"
+
+lemma wf_implies_WF: "wf \<Gamma> M \<Longrightarrow> \<Gamma> \<turnstile> M"
+  by (induction \<Gamma> M rule: wf.induct) auto
+
+thm ABT.induct
+thm wf.induct
+thm lam.wf_abt_wf_args_wf_arg.induct
+
+lemma WF_implies_wf: "\<Gamma> \<turnstile> M \<longrightarrow> wf \<Gamma> M"
+  apply (induction \<Gamma> M rule: lam.wf_abt_wf_args_wf_arg.induct)
+  sorry
+
+inductive reduce :: "Term \<Rightarrow> Term \<Rightarrow> bool" (infix "\<longmapsto>" 50) where
+  beta[intro!]: "(\<lambda> N) \<cdot> M \<longmapsto> N[M]" |
+  appl[intro!]: "L \<longmapsto> L' \<Longrightarrow> L \<cdot> M \<longmapsto> L' \<cdot> M" |
+  appr[intro!]: "M \<longmapsto> M' \<Longrightarrow> L \<cdot> M \<longmapsto> L \<cdot> M'" |
+  abs[intro!]: "N \<longmapsto> N' \<Longrightarrow> \<lambda> N \<longmapsto> \<lambda> N'"
+
+lemma reduce_WF: "\<lbrakk> M \<longmapsto> N; \<Gamma> \<turnstile> M \<rbrakk> \<Longrightarrow> \<Gamma> \<turnstile> N"
+proof (induction arbitrary: \<Gamma> rule: reduce.induct)
+  case (beta N M)
+  have 1: "\<Gamma> \<turnstile> M" using beta by auto
+  have 2: "()#\<Gamma> \<turnstile> N" using beta by auto
+  from 1 2 show ?case apply auto apply (rule lam.subst_pres) apply force 
+    unfolding lam.sub_pres_def \<iota>_def apply auto apply (case_tac x) apply auto done 
+next
+  case (appl L L' M)
+  then show ?case by auto
+next
+  case (appr M M' L)
+  then show ?case by auto
+next
+  case (abs N N' \<Gamma>)
+  have "()#\<Gamma> \<turnstile> N" using abs by auto
+  then have "()#\<Gamma> \<turnstile> N'" using abs by blast
+  then show ?case by auto
+qed
+
+
+section "Confluence"
+
+inductive reduce_parallel :: "Term \<Rightarrow> Term \<Rightarrow> bool" (infix "\<Down>" 50) where
+  pvar[intro!]: "Var x \<Down> Var x" |
+  pabs[intro!]: "N \<Down> N' \<Longrightarrow> \<lambda> N \<Down> \<lambda> N'" |
+  papp[intro!]: "\<lbrakk> L \<Down> L'; M \<Down> M' \<rbrakk> \<Longrightarrow> L \<cdot> M \<Down> L' \<cdot> M'" |
+  pbeta[intro!]: "\<lbrakk> N \<Down> N'; M \<Down> M' \<rbrakk> \<Longrightarrow> (\<lambda> N) \<cdot> M \<Down> N'[M']"
+
+(*
+lemma parallel_refl: "\<Gamma> \<turnstile> M \<Longrightarrow> M \<Down> M"
+  by (induction rule: WF.induct) auto
+*)
+
+lemma beta_parallel: "M \<longmapsto> N \<Longrightarrow> M \<Down> N"
+  apply (induction rule: reduce.induct)
+  sorry
 
 end
