isabelle/Experiment.thy
@@ -1,0 +1,261 @@
+theory Experiment
+  imports Main
+begin
+
+type_synonym var = nat
+type_synonym Renaming = "var \<Rightarrow> var"
+
+fun cons :: "'v \<Rightarrow> (var \<Rightarrow> 'v) \<Rightarrow> (var \<Rightarrow> 'v)" (infixl "\<bullet>" 75) where
+  "(cons v \<sigma>) 0 = v" |
+  "(cons v \<sigma>) (Suc x) = \<sigma> x"
+
+definition lift_ren :: "Renaming \<Rightarrow> Renaming" ("\<Up>") where
+  "\<Up> \<rho> x \<equiv> Suc (\<rho> x)"
+
+(********************************************************************)
+locale substitution =
+  fixes Var :: "var \<Rightarrow> 't"
+    and lift_sub :: "(var \<Rightarrow> 't) \<Rightarrow> (var \<Rightarrow> 't)" ("\<Up>")
+    and ren :: "Renaming \<Rightarrow> (var \<Rightarrow> 't)"
+    and sub :: "(var \<Rightarrow> 't) \<Rightarrow> 't \<Rightarrow> 't"
+    and ids :: "var \<Rightarrow> 't"
+  assumes ren_def: "ren \<rho> x = Var (\<rho> x)"
+    and ren_shift[simp]: "ren (\<Up> \<rho>) = lift_sub (ren \<rho>)"
+    and sub_var[simp]: "sub \<sigma> (Var x) = \<sigma> x"
+    and shift_var[simp]: "\<Up> Var x = Var (Suc x)"
+    and lift_ren_var[simp]: "lift_sub (ren \<rho>) x = Var (Suc (\<rho> x))"
+    and lift_sub_var[simp]: "lift_sub \<sigma> x = sub (ren Suc) (\<sigma> x)"
+    and ids_def: "ids x = Var x"
+begin
+
+lemma ren_cons[simp]: "ren (y \<bullet> \<rho>) = Var y \<bullet> ren \<rho>"
+  apply (rule ext)
+  apply (case_tac x)
+   apply (simp add: ren_def)
+  apply (simp add: ren_def)
+  done
+
+lemma id_sub[simp]: "sub \<sigma> (ids x) = \<sigma> x"
+  unfolding ids_def by simp
+
+lemma ext_id[simp]: "Var 0 \<bullet> \<Up> ids = ids"
+  apply (rule ext) unfolding ids_def ren_def
+  apply (case_tac x) apply force
+  apply (simp add: ren_def)
+  done
+
+definition seq :: "(var \<Rightarrow> 't) \<Rightarrow> (var \<Rightarrow> 't) \<Rightarrow> (var \<Rightarrow> 't)" (infixr ";" 70) where
+  "(\<sigma> ; \<tau>) x \<equiv> sub \<tau> (\<sigma> x)"
+
+theorem shift_ren_seq[simp]: "\<Up> (ren \<rho> ; \<tau>) = (\<Up> (ren \<rho>) ; Var 0 \<bullet> \<Up> \<tau>)"
+  apply (rule ext)
+  apply (case_tac x)
+   apply (simp add: seq_def ren_def)
+   apply (simp add: seq_def ren_def)
+  done
+
+lemma ren_suc[simp]: fixes \<rho>::Renaming shows "(ren \<rho> ; ren Suc) = ren (\<Up> \<rho>)"
+  apply (rule ext)
+  apply (simp add: seq_def ren_def)
+  done
+
+lemma shift_seq_ren[simp]: "ren Suc ; Var 0 \<bullet> \<Up> (ren \<rho>) = ren (\<Up> \<rho>)"
+  apply (rule ext)
+  apply (case_tac x)
+   apply (simp add: seq_def ren_def)
+  apply (simp add: seq_def ren_def )
+  done
+
+end
+(********************************************************************)
+
+datatype Term =
+    Var var
+    | App Term Term (infixl "\<cdot>" 70)
+    | Lam Term      ("\<lambda>")
+
+fun rename :: "Renaming \<Rightarrow> Term \<Rightarrow> Term" where
+  "rename \<rho> (Var x) = Var (\<rho> x)" |
+  "rename \<rho> (L \<cdot> M) = (rename \<rho> L) \<cdot> (rename \<rho> M)" |
+  "rename \<rho> (\<lambda> N) = \<lambda> (rename (0 \<bullet> \<Up> \<rho>) N)"
+
+type_synonym Subst = "var \<Rightarrow> Term"
+
+definition lift_sub :: "Subst \<Rightarrow> Subst" ("\<Up>") where
+  "\<Up> \<sigma> x \<equiv> rename Suc (\<sigma> x)"
+
+fun sub :: "Subst \<Rightarrow> Term \<Rightarrow> Term" where
+  "sub \<sigma> (Var x) = \<sigma> x" |
+  "sub \<sigma> (L \<cdot> M) = (sub \<sigma> L) \<cdot> (sub \<sigma> M)" |
+  "sub \<sigma> (\<lambda> N) = \<lambda> (sub (Var 0 \<bullet> \<Up> \<sigma>) N)"
+
+definition ren :: "Renaming \<Rightarrow> Subst" where
+  "ren \<rho> x \<equiv> Var (\<rho> x)"
+
+lemma rename_sub_ren: "rename \<rho> M = sub (ren \<rho>) M"
+proof (induction M arbitrary: \<rho>)
+  case (Var x)
+then show ?case unfolding ren_def by simp
+next
+  case (App L M)
+  then show ?case by simp
+next
+  case (Lam N)
+  have "ren (0 \<bullet> \<Up> \<rho>) = (Var 0 \<bullet> \<Up> (ren \<rho>))" apply (rule ext)
+    unfolding ren_def lift_ren_def lift_sub_def apply (case_tac x) apply auto done
+  then have "sub (ren (0 \<bullet> \<Up> \<rho>)) N = sub (Var 0 \<bullet> \<Up> (ren \<rho>)) N" by simp
+  with Lam show "rename \<rho> (\<lambda> N) = sub (ren \<rho>) (\<lambda> N)" by simp
+qed
+
+lemma lift_def[simp]: "\<Up> \<sigma> x = sub (ren Suc) (\<sigma> x)"
+  using rename_sub_ren ren_def lift_sub_def by simp
+
+definition ids :: "Subst" where
+  "ids x \<equiv> Var x"
+
+definition seq :: "Subst \<Rightarrow> Subst \<Rightarrow> Subst" (infixr ";" 70) where
+  "(\<sigma> ; \<tau>) x \<equiv> sub \<tau> (\<sigma> x)"
+
+(*
+lemma id_sub[simp]: "sub \<sigma> (ids x) = \<sigma> x"
+  unfolding ids_def by simp
+
+lemma ext_id[simp]: "Var 0 \<bullet> \<Up> ids = ids"
+  apply (rule ext) unfolding ids_def lift_sub_def ren_def
+  apply (case_tac x) apply auto 
+  done
+*)
+
+lemma ren_shift[simp]: "ren (\<Up> \<rho>) = \<Up> (ren \<rho>)"
+  apply (rule ext)
+  apply (case_tac x)
+  apply (simp add: lift_ren_def ren_def)
+  apply (simp add: lift_ren_def ren_def)
+  done
+
+(***********************************************************)
+
+interpretation subst: substitution Var lift_sub ren sub ids
+  apply unfold_locales
+  apply (simp add: ren_def)
+  using ren_shift apply simp
+   apply simp
+   apply (simp add: ren_def)
+   apply (simp add: lift_sub_def ren_def)
+   apply simp
+  apply (simp add: ids_def)
+  done
+
+(***********************************************************)
+
+lemma sub_id[simp]: "sub ids M = M"
+  apply (induction M)
+  apply (simp add: ids_def)
+  apply simp
+   apply simp
+  done
+
+(*
+lemma ren_cons[simp]: "ren (y \<bullet> \<rho>) = Var y \<bullet> ren \<rho>"
+  apply (rule ext)
+  apply (case_tac x)
+   apply (simp add: ren_def)
+  apply (simp add: ren_def)
+  done
+*)
+
+
+
+
+
+theorem ConsSeq[simp]: "(M \<bullet> \<sigma>) ; \<tau> = sub \<tau> M \<bullet> (\<sigma> ; \<tau>)"
+  apply (rule ext)
+  apply (case_tac x)
+   apply (simp add: seq_def)
+   apply (simp add: seq_def)
+  done
+
+theorem shift_ren_seq[simp]: "\<Up> (ren \<rho> ; \<tau>) = (\<Up> (ren \<rho>) ; Var 0 \<bullet> \<Up> \<tau>)"
+  apply (rule ext)
+  apply (case_tac x)
+   apply (simp add: seq_def lift_sub_def ren_def)
+   apply (simp add: seq_def lift_sub_def ren_def)
+  done
+
+lemma ren_sub: "sub \<tau> (sub (ren \<rho>) M) = sub (ren \<rho> ; \<tau>) M"
+  apply (induction M arbitrary: \<tau> \<rho>)
+    apply (simp add: seq_def)
+   apply simp
+  apply simp
+proof -
+  fix M \<tau> \<rho>
+  assume IH: "\<And>\<tau> \<rho>. sub \<tau> (sub (ren \<rho>) M) = sub (ren \<rho> ; \<tau>) M"
+  have "sub (Var 0 \<bullet> \<Up> \<tau>) (sub (Var 0 \<bullet> \<Up> (ren \<rho>)) M)
+        = sub (Var 0 \<bullet> \<Up> \<tau>) (sub (ren (0 \<bullet> \<Up> \<rho>)) M)" by simp
+  also have "... = sub (ren (0 \<bullet> \<Up> \<rho>) ; Var 0 \<bullet> \<Up> \<tau>) M" using IH by fast
+  also have "... = sub (Var 0 \<bullet> (\<Up> (ren \<rho>) ; Var 0 \<bullet> \<Up> \<tau>)) M" by simp
+  finally show "sub (Var 0 \<bullet> \<Up> \<tau>) (sub (Var 0 \<bullet> \<Up> (ren \<rho>)) M) 
+               = sub (Var 0 \<bullet> (\<Up> (ren \<rho>) ; Var 0 \<bullet> \<Up> \<tau>)) M" .
+qed
+
+lemma ren_suc[simp]: fixes \<rho>::Renaming shows "(ren \<rho> ; ren Suc) = ren (\<Up> \<rho>)"
+  apply (rule ext)
+  apply (simp add: seq_def ren_def)
+  done
+
+lemma shift_seq_ren[simp]: "ren Suc ; Var 0 \<bullet> \<Up> (ren \<rho>) = ren (\<Up> \<rho>)"
+  apply (rule ext)
+  apply (case_tac x)
+   apply (simp add: seq_def ren_def)
+  apply (simp add: seq_def ren_def )
+  done
+
+lemma shift_sub_ren[simp]: "\<Up> (\<sigma> ; ren \<rho>) = (\<Up> \<sigma> ; Var 0 \<bullet> ren (\<Up> \<rho>) )"
+  apply (rule ext)
+  apply (case_tac x)
+   apply (simp add: seq_def ren_def ren_sub)
+   apply (simp add: seq_def ren_def ren_sub)
+  done
+
+lemma sub_ren: "sub (ren \<rho>) (sub \<sigma> M) = sub (\<sigma> ; ren \<rho>) M"
+  apply (induction M arbitrary: \<sigma> \<rho>)
+    apply (simp add: seq_def)
+   apply simp
+  apply simp
+proof -
+  fix M \<sigma> \<rho> 
+  assume IH: "\<And>\<sigma> \<rho>. sub (ren \<rho>) (sub \<sigma> M) = sub (\<sigma> ; ren \<rho>) M"
+  have "sub (Var 0 \<bullet> \<Up> (ren \<rho>)) (sub (Var 0 \<bullet> \<Up> \<sigma>) M)
+        = sub (ren (0 \<bullet> \<Up> \<rho>)) (sub (Var 0 \<bullet> \<Up> \<sigma>) M)" by simp
+  also have "... = sub ((Var 0 \<bullet> \<Up> \<sigma>) ; ren (0 \<bullet> \<Up> \<rho>)) M" using IH by fast
+  also have "... = sub (Var 0 \<bullet> (\<Up> \<sigma> ; Var 0 \<bullet> \<Up> (ren \<rho>))) M" by simp
+  finally show "sub (Var 0 \<bullet> \<Up> (ren \<rho>)) (sub (Var 0 \<bullet> \<Up> \<sigma>) M) 
+        = sub (Var 0 \<bullet> (\<Up> \<sigma> ; Var 0 \<bullet> \<Up> (ren \<rho>))) M" .
+qed
+
+lemma sub_suc[simp]: fixes \<rho>::Renaming shows "(\<sigma> ; ren Suc) = \<Up> \<sigma>"
+  unfolding seq_def lift_sub_def apply (rule ext) using rename_sub_ren apply simp done
+
+lemma shift_seq_sub[simp]: "ren Suc ; Var 0 \<bullet> \<Up> \<sigma> = \<Up> \<sigma>"
+  apply (rule ext) apply (case_tac x) 
+   apply (simp add: seq_def ren_def)
+   apply (simp add: seq_def ren_def)
+  done
+
+lemma sub_sub: "sub \<tau> (sub \<sigma> M) = sub (\<sigma> ; \<tau>) M"
+proof (induction M arbitrary: \<sigma> \<tau>)
+  case (Var x)
+  then show ?case by (simp add: seq_def)
+next
+  case (Lam M)
+  have "Var 0 \<bullet> \<Up> \<sigma> ; Var 0 \<bullet> \<Up> \<tau> = Var 0 \<bullet> \<Up> (\<sigma> ; \<tau>)"
+    apply (rule ext) apply (case_tac x) 
+     apply (simp add: seq_def lift_sub_def)
+    apply simp apply (simp add: seq_def lift_sub_def ren_sub) using sub_ren apply auto done
+  with Lam show ?case by simp
+next
+  case (App L M)
+  then show ?case by simp
+qed
+
+end
